theories/typing/function.v
@@ -1,6 +1,5 @@
 From iris.base_logic Require Import big_op.
 From iris.proofmode Require Import tactics.
-From iris.program_logic Require Import hoare.
 From lrust.lifetime Require Import borrow.
 From lrust.typing Require Export type.
 From lrust.typing Require Import programs.
@@ -117,13 +116,15 @@ Section fn.
     - (* TODO: The IH is not usable here. What we really want is to do induction over "how many of the arguments still need to be evaluated", so the base case has all the ps evaluated and the inductive case evaluates one of them. *)
   Abort.
 
-  Lemma typed_fn {A n} E L T E' (tys : A → vec type n) ty fb kb
-        (argsb : vec binder n) ef e `{!CopyC T, !SendC T} :
+  Lemma typed_fn {A n m} E L E' (tys : A → vec type n) ty fb kb (argsb : vec binder n) ef e
+       (cps : vec path m) (ctyl : vec type m) `{!LstCopy ctyl, !LstSend ctyl} :
     ef = Rec fb (kb :: argsb) e → Closed (fb :b: kb :b: argsb +b+ []) e →
     (∀ x f k (args : vec val n), typed_body (E' x) [] [CctxElt k [] 1 (λ v, [TCtx_hasty (v!!!0) (ty x)])]
-                 (TCtx_hasty f (fn E' tys ty) :: zip_with (TCtx_hasty ∘ of_val) args (tys x) ++ T)
+                 (TCtx_hasty f (fn E' tys ty) ::
+                  zip_with (TCtx_hasty ∘ of_val) args (tys x) ++
+                  zip_with TCtx_hasty cps ctyl)
                  (subst' fb f $ subst_vec (kb ::: argsb) (Vector.map of_val $ k ::: args) e)) →
-    typed_instruction_ty E L T ef (fn E' tys ty).
+    typed_instruction_ty E L (zip_with TCtx_hasty cps ctyl) ef (fn E' tys ty).
   Proof.
     iIntros (-> Hc Hbody). iIntros (tid qE) "!# #LFT $ $ #HT". iApply wp_value.
     { simpl. rewrite decide_left. done. }
@@ -137,6 +138,6 @@ Section fn.
     rewrite [elctx_interp]lock [llctx_interp]lock [tctx_interp]lock.
     wp_rec. unlock. subst eb. iApply (Hbody with "* LFT HE HL HC").
     rewrite tctx_interp_cons tctx_interp_app. iFrame "HT' IH".
-    iApply sendc_change_tid. done.
+    iApply tctx_send. done.
   Qed.
 End fn.
